WIP

security/Backtranslation.v
@@ -567,7 +567,133 @@ Section Backtranslation.
       econstructor 1.
     Qed.
 
+    Lemma code_of_event_step_call_internal
+          ev
+          cp cp' id vs
+          p f k e le m
+          ge
+          (GE: ge = globalenv p)
+          (EV: ev = Event_call cp cp' id vs)
+          (* bt should ensure them *)
+          (GLOB: e ! id = None)
+          b
+          (FINDB: Genv.find_symbol ge id = Some b)
+          fd
+          (FINDF: Genv.find_funct ge (Vptr b Ptrofs.zero) = Some fd)
+          (TYPEF: type_of_fundef fd = Tfunction (list_eventval_to_typelist vs) Tvoid cc_default)
+          (WFARGS: Forall (wf_eventval ge e) vs)
+          f1
+          (INTERNAL: fd = Internal f1)
+          (* asm should ensure them *)
+          (NPTR: Forall not_ptr (list_eventval_to_list_val ge vs))
+          (CP1: cp = comp_of f)
+          (CP2: cp' = comp_of fd)
+          (CROSS: Genv.type_of_call ge (comp_of f) (comp_of fd) = Genv.CrossCompartmentCall)
+          (ALLOW: Genv.allowed_cross_call ge (comp_of f) (Vptr b Ptrofs.zero))
+          (* handle during proof *)
+          e1 le1 m1
+          (ENTRY: function_entry1 ge f1 (list_eventval_to_list_val ge vs) m e1 le1 m1)
+      :
+        Star (Clight.semantics1 p)
+             (State f (code_of_event ev) k e le m)
+             (ev :: nil)
+             (State f1 (fn_body f1) (Kcall None f e le k) e1 le1 m1).
+    Proof.
+      subst; simpl. unfold code_of_call.
+      econstructor 2.
+      3:{ rewrite E0_right. reflexivity. }
+      { eapply step_call; simpl; eauto.
+        { eapply eval_Elvalue.
+          - eapply eval_Evar_global; eauto.
+          - eapply deref_loc_reference. auto.
+        }
+        { eapply list_eventval_to_expr_val_eval. eapply Forall_impl. 2: eauto. intros. apply wf_eventval_weak_weak; auto. }
+        red; auto.
+        unfold Genv.find_comp. setoid_rewrite FINDF.
+        eapply call_trace_cross; eauto. apply Genv.find_invert_symbol; auto.
+        eapply (list_eventval_to_expr_val_match (globalenv p)); eauto.
+      }
+      econstructor 2.
+      3:{ rewrite E0_right. reflexivity. }
+      { eapply step_internal_function; eauto. }
+      econstructor 1.
+    Qed.
+
+    Lemma code_of_event_step_call_external
+          ev
+          cp cp' id vs
+          p f k e le m
+          ge
+          (GE: ge = globalenv p)
+          (EV: ev = Event_call cp cp' id vs)
+          (* bt should ensure them *)
+          (GLOB: e ! id = None)
+          b
+          (FINDB: Genv.find_symbol ge id = Some b)
+          fd
+          (FINDF: Genv.find_funct ge (Vptr b Ptrofs.zero) = Some fd)
+          (TYPEF: type_of_fundef fd = Tfunction (list_eventval_to_typelist vs) Tvoid cc_default)
+          (WFARGS: Forall (wf_eventval ge e) vs)
+          ef0 targs0 tres0 cconv0
+          (EXTERNAL: fd = External ef0 targs0 tres0 cconv0)
+          (* asm should ensure them *)
+          (NPTR: Forall not_ptr (list_eventval_to_list_val ge vs))
+          (CP1: cp = comp_of f)
+          (CP2: cp' = comp_of fd)
+          (CROSS: Genv.type_of_call ge (comp_of f) (comp_of fd) = Genv.CrossCompartmentCall)
+          (ALLOW: Genv.allowed_cross_call ge (comp_of f) (Vptr b Ptrofs.zero))
+          (* handle during proof *)
+          sev sname sargs svr
+          (SYSEV: sev = Event_syscall sname sargs svr)
+          vres m1
+          (SEM: external_call ef0 ge (comp_of f) (list_eventval_to_list_val ge vs) m (sev :: nil) vres m1)
+      :
+        Star (Clight.semantics1 p)
+             (State f (code_of_event ev) k e le m)
+             (ev :: sev :: nil)
+             (Returnstate vres (Kcall None f e le k) m1 (rettype_of_type tres0) (comp_of ef0)).
+    Proof.
+      subst; simpl. unfold code_of_call.
+      econstructor 2.
+      3:{ rewrite E0_right. reflexivity. }
+      { eapply step_call; simpl; eauto.
+        { eapply eval_Elvalue.
+          - eapply eval_Evar_global; eauto.
+          - eapply deref_loc_reference. auto.
+        }
+        { eapply list_eventval_to_expr_val_eval. eapply Forall_impl. 2: eauto. intros. apply wf_eventval_weak_weak; auto. }
+        red; auto.
+        unfold Genv.find_comp. setoid_rewrite FINDF.
+        eapply call_trace_cross; eauto. apply Genv.find_invert_symbol; auto.
+        eapply (list_eventval_to_expr_val_match (globalenv p)); eauto.
+      }
+      econstructor 2.
+      3:{ rewrite E0_right. reflexivity. }
+      { eapply step_internal_function; eauto. }
+      econstructor 1.
+    Qed.
+
     (* TODO *)
+
+  | step_call : forall (f : function) (optid : option ident) (a : expr) (al : list expr) (k : cont) (e : env) (le : temp_env) (m : mem) (tyargs : typelist) (tyres : type) (cconv : calling_convention)
+                  (vf : val) (vargs : list val) (fd : fundef) (t : trace),
+                Cop.classify_fun (typeof a) = Cop.fun_case_f tyargs tyres cconv ->
+                eval_expr ge e (comp_of f) le m a vf ->
+                eval_exprlist ge e (comp_of f) le m al tyargs vargs ->
+                Genv.find_funct ge vf = Some fd ->
+                type_of_fundef fd = Tfunction tyargs tyres cconv ->
+                Genv.allowed_call ge (comp_of f) vf ->
+                (Genv.type_of_call ge (comp_of f) (Genv.find_comp ge vf) = Genv.CrossCompartmentCall -> Forall not_ptr vargs) ->
+                call_trace ge (comp_of f) (Genv.find_comp ge vf) vf vargs (typlist_of_typelist tyargs) t ->
+                step ge function_entry (State f (Scall optid a al) k e le m) t (Callstate fd vargs (Kcall optid f e le k) m)
+
+    Definition code_of_call (cp cp': compartment) (id: ident) (vs: list eventval) :=
+      Scall None (Evar id (Tfunction (list_eventval_to_typelist vs) Tvoid cc_default)) (list_eventval_to_list_expr vs).
+
+    match e with
+      | Event_syscall name vs v => code_of_syscall name vs v
+      | Event_return cp cp' v => code_of_return cp cp' v
+      end.
 
 
   End CODE.
